lean/BPlusTree.lean
@@ -1,6 +1,8 @@
+import BPlusTree.Model.Spec
 import BPlusTree.Model.Leaf
 import BPlusTree.Model.Branch
 import BPlusTree.Model.Tree
 import BPlusTree.Proofs.Leaf
+import BPlusTree.Proofs.Spec
 import BPlusTree.Proofs.Branch
 import BPlusTree.Proofs.Tree
